Progress with [mfix] and [handle].

theories/handle.v
@@ -1,10 +1,10 @@
-From ExtLib.Structures Require Export Monads MonadLaws.
-Require Import lang eval.
+Require Import lang eval monads.
 Require free.
 
-Section Handle.
+(* This file defines an interpretation (a transformation) of the [free]
+   monad into a monad equipped with [mzero] and [mfix] combinators. *)
 
-(* Suppose the target monad has [mzero] and [mfix]. *)
+Section Handle.
 
 Variable target : Type → Type.
 Variable M : Monad target.
@@ -14,11 +14,15 @@ Variable MZL : MonadZeroLaws M MZ.
 Variable MF : MonadFix target.
 Variable MFL : MonadFixLaws MF.
 
+Section A.
+
+Context {A : Type}.
+
 (* ------------------------------------------------------------------------ *)
 
 (* An interpretation of our free monad into the target monad. *)
 
-Definition handle_pre {A}
+Definition handle_pre
   (handle : free.mon A → target A)
   (m : free.mon A) : target A
 :=
@@ -43,47 +47,49 @@ Definition handle_pre {A}
       end
   end.
 
-Definition handle {A} : free.mon A → target A :=
+Definition handle : free.mon A → target A :=
   mfix handle_pre.
 
-Lemma fixed_point {A} (m : free.mon A) :
-  mleq eq (handle m) (handle_pre handle m).
+Lemma handle_fixed_point :
+  handle = handle_pre handle.
 Proof.
-  eapply mfix_monotonic. reflexivity.
+  eapply mfix_fixed_point.
+  (* We must check that [handle_pre] is monotonic. *)
+  intros self1 self2 Hself m.
+  destruct m; simpl;
+  eauto using mleq_reflexive.
+  destruct req; eauto.
 Qed.
-
-(* TODO we would like to deduce this: *)
-
-Lemma fp {A} (m : free.mon A) :
-  handle m = handle_pre handle m.
-Proof.
-Admitted.
 
 (* Paraphrase lemmas. *)
 
-Lemma handle_ret {A} (a : A) :
+Lemma handle_ret (a : A) :
   handle (free.Ret a) = ret a.
 Proof.
-  rewrite fp. reflexivity.
+  rewrite handle_fixed_point. reflexivity.
 Qed.
 
-Lemma handle_fail {A} :
+Lemma handle_fail :
   handle (free.Fail : free.mon A) = mzero.
 Proof.
-  rewrite fp. reflexivity.
+  rewrite handle_fixed_point. reflexivity.
 Qed.
 
-Lemma handle_next {A} :
+Lemma handle_next :
   handle (free.Next : free.mon A) = mzero.
 Proof.
-  rewrite fp. reflexivity.
+  rewrite handle_fixed_point. reflexivity.
 Qed.
 
-Lemma handle_stop {A} η e (k : val → free.mon A) :
+Lemma handle_stop η e (k : val → free.mon A) :
   handle (free.Stop (free.REval η e) k) = handle (bind (eval η e) k).
 Proof.
-  rewrite fp. reflexivity.
+  rewrite handle_fixed_point. (* rewrites both occurrences... *)
+  simpl. rewrite <- handle_fixed_point.       (* rewrite back *)
+  reflexivity.
 Qed.
+
+End A.
 
 (* ------------------------------------------------------------------------ *)
 
