theories/monads.v
@@ -1,0 +1,29 @@
+From ExtLib.Structures Require Export Monads MonadLaws.
+
+(* The type class MonadFix in coq-ext-lib does not work for us,
+   so we replace it with the following class. *)
+
+Section MonadFixLaws.
+
+  Context {m : Type -> Type}.
+  Context (MF : MonadFix m).
+
+  Class MonadFixLaws :=
+    {
+      mleq :
+        forall {A}, m A -> m A -> Prop;
+      mleq_reflexive :
+        forall {A} (m : m A),
+        mleq m m;
+      mleq_transitive :
+        forall {A} (m1 m2 m3 : m A),
+        mleq m1 m2 -> mleq m2 m3 -> mleq m1 m3;
+      mfix_fixed_point :
+        forall {T A} (ff : (T -> m A) -> (T -> m A)),
+        (forall p1 p2,
+          (forall t, mleq (p1 t) (p2 t)) ->
+          (forall t, mleq (ff p1 t) (ff p2 t))) ->
+        mfix ff = ff (mfix ff)
+    }.
+
+End MonadFixLaws.
